add infrastructures for argument substitution in predicate body

vipersemcommon/PredicatesUtil.thy
@@ -16,7 +16,7 @@ fun real_mult_permexpr :: "real \<Rightarrow> pure_exp exp_or_wildcard \<Rightar
   | "real_mult_permexpr p (PureExp e) = PureExp (Binop (real_to_expr p) Mult e)"
 
 fun syntactic_mult :: "real \<Rightarrow> assertion \<Rightarrow> assertion"
-  where 
+  where
     "syntactic_mult p (Atomic (Pure e)) = (Atomic (Pure e))"
   | "syntactic_mult p (Atomic (Acc e_r f e_p)) = (Atomic (Acc e_r f (real_mult_permexpr p e_p)))"
   | "syntactic_mult p (Atomic (AccPredicate pred_id e_args e_p)) = 
@@ -29,5 +29,39 @@ fun syntactic_mult :: "real \<Rightarrow> assertion \<Rightarrow> assertion"
   | "syntactic_mult p (ImpureOr A B) = ImpureOr (syntactic_mult p A) (syntactic_mult p B)"
   | "syntactic_mult p (A --* B) = (syntactic_mult p A) --* (syntactic_mult p B)"
   | "syntactic_mult p (CondAssert e A B) = CondAssert e (syntactic_mult p A) (syntactic_mult p B)"
+
+hide_const predicate_decl.args function_decl.args method_decl.args
+fun substitute_args_expr :: "pure_exp \<Rightarrow> pure_exp list \<Rightarrow> pure_exp" where
+    "substitute_args_expr (Var x) args = args ! x"
+  | "substitute_args_expr (Unop uop e) args = Unop uop (substitute_args_expr e args)"
+  | "substitute_args_expr (Binop e1 bop e2) args = Binop (substitute_args_expr e1 args) bop (substitute_args_expr e2 args)"
+  | "substitute_args_expr (CondExp cond e1 e2) args = CondExp (substitute_args_expr cond args) (substitute_args_expr e1 args) (substitute_args_expr e2 args)"
+  | "substitute_args_expr (FieldAcc e f) args = FieldAcc (substitute_args_expr e args) f"
+  | "substitute_args_expr (Unfolding pid es e) args = Unfolding pid (map (\<lambda>e. substitute_args_expr e args) es) (substitute_args_expr e args)"
+  | "substitute_args_expr e _ = e"
+
+fun substitute_args_assertion :: "assertion \<Rightarrow> pure_exp list \<Rightarrow> assertion" where
+    "substitute_args_assertion (Atomic (Pure e)) args = Atomic (Pure (substitute_args_expr e args))"
+  | "substitute_args_assertion (Atomic (Acc e_r f (PureExp e_p))) args = Atomic (Acc (substitute_args_expr e_r args) f (PureExp (substitute_args_expr e_p args)))"
+  | "substitute_args_assertion (Atomic (Acc e_r f Wildcard)) args = Atomic (Acc (substitute_args_expr e_r args) f Wildcard)"
+  | "substitute_args_assertion (Atomic (AccPredicate pid e_args (PureExp e_p))) args = Atomic (AccPredicate pid e_args (PureExp (substitute_args_expr e_p args)))"
+  | "substitute_args_assertion (Atomic (AccPredicate pid e_args Wildcard)) args = Atomic (AccPredicate pid e_args Wildcard)"
+  | "substitute_args_assertion (Imp e A) args = Imp (substitute_args_expr e args) (substitute_args_assertion A args)"
+  | "substitute_args_assertion (Star A B) args = Star (substitute_args_assertion A args) (substitute_args_assertion B args)"
+  | "substitute_args_assertion (CondAssert e A B) args = CondAssert (substitute_args_expr e args) (substitute_args_assertion A args) (substitute_args_assertion B args)"
+  | "substitute_args_assertion A _ = A"
+
+lemma substitute_synmult_commute:
+  assumes "p \<ge> 0"
+  shows "substitute_args_assertion (syntactic_mult p A) args = syntactic_mult p (substitute_args_assertion A args)"
+  using assms
+  apply (induction A; simp?)
+  apply (rename_tac atm)
+  apply (case_tac atm; simp?)
+   apply (rename_tac e_r f perm)
+   apply (case_tac perm; simp?)
+  apply (rename_tac pid e_args perm)
+  apply (case_tac perm; simp?)
+  done
 
 end
